fstar/test/MLS.Test.FromExt.Welcome.fst
@@ -29,10 +29,8 @@ let test_welcome_one t =
   | Success cs -> begin
     let cb = mk_concrete_crypto_bytes cs in
 
-    let init_priv = hex_string_to_bytes t.init_priv in
-    let init_priv: hpke_private_key bytes = if length init_priv = hpke_private_key_length #bytes then init_priv else failwith "test_welcome_one: bad private key length" in
-    let signer_pub = hex_string_to_bytes t.signer_pub in
-    let signer_pub: sign_public_key bytes = if length signer_pub = sign_public_key_length #bytes then signer_pub else failwith "test_welcome_one: bad public key length" in
+    let init_priv = extract_result (mk_hpke_private_key (hex_string_to_bytes t.init_priv) "test_welcome_one" "init_priv") in
+    let signer_pub = extract_result (mk_sign_public_key (hex_string_to_bytes t.signer_pub) "test_welcome_one" "signer_pub") in
     let key_package: key_package_nt bytes tkt =
       match parse (mls_message_nt bytes) (hex_string_to_bytes t.key_package) with
       | None -> failwith "test_welcome_one: malformed key package"
