fstar/treedem/MLS.TreeDEM.Message.Transcript.fst
@@ -10,9 +10,8 @@ val compute_confirmed_transcript_hash:
   wire_format_nt -> framed_content_nt bytes -> bytes -> bytes ->
   result (lbytes bytes (hash_length #bytes))
 let compute_confirmed_transcript_hash #bytes #cb wire_format msg signature interim_transcript_hash =
-  if not (length signature < pow2 30) then
-    internal_failure "compute_confirmed_transcript_hash: signature too long"
-  else if not (msg.content.content_type = CT_commit) then
+  let? signature = mk_mls_bytes signature "compute_confirmed_transcript_hash" "signature" in
+  if not (msg.content.content_type = CT_commit) then
     internal_failure "compute_confirmed_transcript_hash: should only be used on a commit message"
   else (
     let serialized_msg = serialize (confirmed_transcript_hash_input_nt bytes) ({
@@ -30,13 +29,10 @@ val compute_interim_transcript_hash:
   bytes -> bytes ->
   result (lbytes bytes (hash_length #bytes))
 let compute_interim_transcript_hash #bytes #cb confirmation_tag confirmed_transcript_hash =
-  if not (length confirmation_tag < pow2 30) then
-    internal_failure "compute_interim_transcript_hash: confirmation_tag too long"
-  else (
-    let serialized_auth = serialize (interim_transcript_hash_input_nt bytes) ({
-      confirmation_tag;
-    }) in
-    let hash_input = concat #bytes confirmed_transcript_hash serialized_auth in
-    if not (length hash_input < hash_max_input_length #bytes) then error ""
-    else return (hash_hash hash_input)
-  )
+  let? confirmation_tag = mk_mls_bytes confirmation_tag "compute_interim_transcript_hash" "confirmation_tag" in
+  let serialized_auth = serialize (interim_transcript_hash_input_nt bytes) ({
+    confirmation_tag;
+  }) in
+  let hash_input = concat #bytes confirmed_transcript_hash serialized_auth in
+  if not (length hash_input < hash_max_input_length #bytes) then error ""
+  else return (hash_hash hash_input)
